pcuic/theories/PCUICSubstitution.v
@@ -1120,31 +1120,7 @@ Proof.
   revert Δ; induction Γ as [|[na [b|] ty]]; intros Δ; simpl; auto.
 Qed.
 
-
-(* Smashing a context Γ with Δ depending on it is the same as smashing Γ
-     and substituting all references to Γ in Δ by the expansions of let bindings.
-  *)
-
 Arguments Nat.sub : simpl nomatch.
-
-Fixpoint extended_subst (Γ : context) (n : nat) 
-  (* Δ, smash_context Γ, n |- extended_subst Γ n : Γ *) :=
-  match Γ with
-  | nil => nil
-  | cons d vs =>
-    match decl_body d with
-    | Some b =>
-      (* Δ , vs |- b *)
-      let s := extended_subst vs n in
-      (* Δ , smash_context vs , n |- s : vs *)
-      let b' := lift (context_assumptions vs + n) #|s| b in
-      (* Δ, smash_context vs, n , vs |- b' *)
-      let b' := subst0 s b' in
-      (* Δ, smash_context vs , n |- b' *)
-      b' :: s
-    | None => tRel n :: extended_subst vs (S n)
-    end
-  end.
 
 Lemma extended_subst_length Γ n : #|extended_subst Γ n| = #|Γ|.
 Proof.
