pcuic/theories/PCUICTyping.v
@@ -816,7 +816,9 @@ Module PCUICTypingDef <: Typing PCUICTerm PCUICEnvironment PCUICEnvTyping.
   Definition conv := @conv.
   Definition cumul := @cumul.
   Definition smash_context := smash_context.
+  Definition extended_subst := extended_subst.
   Definition lift_context := lift_context.
+  Definition subst_context := subst_context.  
   Definition subst_telescope := subst_telescope.
   Definition subst_instance_context := subst_instance_context.
   Definition subst_instance_constr := subst_instance_constr.
