template-coq/theories/Typing.v
@@ -893,6 +893,8 @@ Module TemplateTyping <: Typing TemplateTerm TemplateEnvironment TemplateEnvTypi
   Definition lift := lift.
   Definition subst := subst.
   Definition lift_context := lift_context.
+  Definition subst_context := subst_context.
+  Definition extended_subst := extended_subst.
   Definition subst_instance_constr := subst_instance_constr.
   Definition subst_instance_context := subst_instance_context.
   Definition subst_telescope := subst_telescope.
