pcuic/theories/PCUICConversion.v
@@ -2466,6 +2466,20 @@ Proof.
   rewrite !lift_closed in X => //.
 Qed.
 
+Lemma weaken_cumul {cf:checker_flags} {Σ Γ t u} Δ : 
+  wf Σ.1 -> closedn_ctx 0 Γ ->
+  closedn #|Γ| t -> closedn #|Γ| u ->
+  Σ ;;; Γ |- t <= u ->
+  Σ ;;; Δ ,,, Γ |- t <= u.
+Proof.
+  intros wfΣ clΓ clt clu ty.
+  epose proof (weakening_cumul Σ [] Γ Δ t u wfΣ).
+  rewrite !app_context_nil_l in X.
+  forward X by eauto.
+  rewrite closed_ctx_lift in X; auto.
+  rewrite !lift_closed in X => //.
+Qed.
+
 Lemma conv_subst_instance {cf:checker_flags} (Σ : global_env_ext) Γ u A B univs :
   forallb (fun x => negb (Level.is_prop x)) u ->
   valid_constraints (global_ext_constraints (Σ.1, univs))
@@ -2752,14 +2766,14 @@ Proof.
   eapply subst_conv; eauto.
 Qed.
 
-Lemma cumul_ctx_subst {cf:checker_flags} Σ Γ Γ' Δ Δ' s s' : 
+Lemma cumul_ctx_subst {cf:checker_flags} Σ Γ Γ' Γ'0 Γ'' Δ Δ' s s' : 
   wf Σ.1 ->
-  wf_local Σ (Γ ,,, Γ' ,,, Δ) ->
-  cumul_ctx_rel Σ (Γ ,,, Γ') Δ Δ' ->
-  All2 (conv Σ []) s s' ->
-  subslet Σ [] s Γ ->
-  subslet Σ [] s' Γ ->
-  cumul_ctx_rel Σ (subst_context s 0 Γ') (subst_context s #|Γ'| Δ) (subst_context s' #|Γ'| Δ').
+  wf_local Σ (Γ ,,, Γ' ,,, Γ'' ,,, Δ) ->
+  cumul_ctx_rel Σ (Γ ,,, Γ' ,,, Γ'') Δ Δ' ->
+  All2 (conv Σ Γ) s s' ->
+  untyped_subslet Γ s Γ' ->
+  untyped_subslet Γ s' Γ'0 ->
+  cumul_ctx_rel Σ (Γ ,,, subst_context s 0 Γ'') (subst_context s #|Γ''| Δ) (subst_context s' #|Γ''| Δ').
 Proof.
   intros wfΣ wf. induction 1.
   - simpl. constructor.
@@ -2769,11 +2783,10 @@ Proof.
     specialize (IHX wf Hs subs subs').
     constructor; auto. 
     red. red in p. simpl.
-    epose proof (subst_cumul [] Γ Γ (Γ' ,,, Γ0) _ _ _ _ wfΣ subs subs' Hs).
-    rewrite app_context_nil_l app_context_assoc in X0.
+    epose proof (untyped_subst_cumul Γ Γ' Γ'0 (Γ'' ,,, Γ0) _ _ _ _ wfΣ subs subs' Hs).
+    rewrite app_context_assoc in X0.
     specialize (X0 wf p).
-    rewrite subst_context_app in X0; autorewrite with len in X0.
-    rewrite app_context_nil_l in X0.
+    rewrite !subst_context_app app_context_assoc in X0; autorewrite with len in X0.
     now rewrite -(All2_local_env_length X).
   - rewrite !subst_context_snoc /=.
     intros Hs subs subs'.
@@ -2782,13 +2795,13 @@ Proof.
     constructor; auto.
     red. red in p. simpl.
     destruct p as [pb pt].
-    epose proof (subst_cumul [] Γ Γ (Γ' ,,, Γ0) _ _ _ _ wfΣ subs subs' Hs) as X0.
-    rewrite app_context_nil_l app_context_assoc in X0.
+    epose proof (untyped_subst_cumul Γ Γ' Γ'0 (Γ'' ,,, Γ0) _ _ _ _ wfΣ subs subs' Hs) as X0.
+    rewrite app_context_assoc in X0.
     specialize (X0 wf pb).
-    epose proof (subst_cumul [] Γ Γ (Γ' ,,, Γ0) _ _ _ _ wfΣ subs subs' Hs) as X1.
-    rewrite app_context_nil_l app_context_assoc in X1.
+    epose proof (untyped_subst_cumul Γ Γ' Γ'0 (Γ'' ,,, Γ0) _ _ _ _ wfΣ subs subs' Hs) as X1.
+    rewrite !app_context_assoc in X1.
     specialize (X1 wf pt).
-    rewrite !subst_context_app !app_context_nil_l in X0, X1; autorewrite with len in X0, X1.
+    rewrite !subst_context_app !app_context_assoc in X0, X1; autorewrite with len in X0, X1.
     now rewrite -(All2_local_env_length X).
 Qed.
 
@@ -2810,4 +2823,55 @@ Proof.
       destruct (IHX _ _ Hnth) as [decl' [Hnth' cum]].
       eexists; intuition eauto.
   - move=> H; elimtype False; depelim H; simpl in H0; noconf H0.
+Qed.
+
+Require Import ssrbool.
+
+Lemma closed_ctx_decl k d Γ : closedn_ctx k (d :: Γ) =
+  closed_decl (k + #|Γ|) d && closedn_ctx k Γ.
+Proof.
+  unfold closedn_ctx at 1.
+  rewrite mapi_rev /= forallb_app {2}/id /= andb_true_r.
+  replace (#|Γ| - 0) with #|Γ| by lia.
+  rewrite andb_comm. f_equal.
+  unfold closedn_ctx.
+  rewrite mapi_rev (mapi_rec_add _ _ 1 0) /=.
+  f_equal.
+Qed.
+
+Lemma weaken_cumul_ctx {cf:checker_flags} Σ Γ Γ' Δ Δ' :
+  wf Σ.1 ->
+  closed_ctx (Γ' ,,, Δ) ->
+  closed_ctx (Γ' ,,, Δ') ->
+  wf_local Σ Γ ->
+  cumul_ctx_rel Σ Γ' Δ Δ' ->
+  cumul_ctx_rel Σ (Γ ,,, Γ') Δ Δ'.
+Proof.
+  intros wfΣ wf wf' wf''. induction 1.
+  - simpl. constructor.
+  - rewrite /= closed_ctx_decl in wf.
+    rewrite /= closed_ctx_decl in wf'.
+    move/andP: wf => [wfd wf].
+    move/andP: wf' => [wfd' wf'].
+    constructor; auto.
+    + now eapply IHX.
+    + red. red in p. 
+      rewrite -app_context_assoc.
+      eapply weaken_cumul; eauto.
+      autorewrite with len; simpl; rewrite (All2_local_env_length X).
+      now autorewrite with len in wfd'.
+  - rewrite /= closed_ctx_decl in wf.
+    rewrite /= closed_ctx_decl in wf'.
+    move/andP: wf => [wfd wf].
+    move/andP: wf' => [wfd' wf'].
+    constructor; auto.
+    + now eapply IHX.
+    + red. red in p. 
+      rewrite -app_context_assoc.
+      autorewrite with len in *.
+      destruct p.
+      move/andP: wfd => /= [wfb wft].
+      move/andP: wfd' => /= [wfb' wft'].
+      rewrite <- (All2_local_env_length X) in *.
+      split; eapply weaken_cumul; autorewrite with len; eauto.
 Qed.
